WIP adapt monotonicity and weakening lemmas

theories/logrel/ftlr/interp_weakening.v
@@ -23,6 +23,56 @@ Section fundamental.
   Implicit Types w : (leibnizO Word).
   Implicit Types interp : (V).
 
+  Lemma filter_heap_map W (f : Word -> Word) w :
+    heap_authority_base (f w) = heap_authority_base w ->
+    clear_tag (f w) = f (clear_tag w) ->
+    filter_heap W (f w) = f (filter_heap W w).
+  Proof.
+    intros Hbase Hclear. rewrite /filter_heap Hbase.
+    destruct (heap_authority_base w) as [b|]; last done.
+    destruct (heap_lookup_addr (heap_std W) b) as [ [base obj] | ]; last done.
+    cbn. destruct (alloc_object_status obj); done.
+  Qed.
+
+  Lemma filter_heap_borrow W w :
+    filter_heap W (borrow w) = borrow (filter_heap W w).
+  Proof.
+    apply filter_heap_map;
+      destruct w as [z|[t p g b e a|t p g b e a]|t p g b e a|ot [t p g b e a|t p g b e a] ];
+      reflexivity.
+  Qed.
+
+  Lemma filter_heap_deeplocal W w :
+    filter_heap W (deeplocal w) = deeplocal (filter_heap W w).
+  Proof.
+    apply filter_heap_map;
+      destruct w as [z|[t p g b e a|t p g b e a]|t p g b e a|ot [t p g b e a|t p g b e a] ];
+      reflexivity.
+  Qed.
+
+  Lemma filter_heap_readonly W w :
+    filter_heap W (readonly w) = readonly (filter_heap W w).
+  Proof.
+    apply filter_heap_map;
+      destruct w as [z|[t p g b e a|t p g b e a]|t p g b e a|ot [t p g b e a|t p g b e a] ];
+      reflexivity.
+  Qed.
+
+  Lemma filter_heap_force_global W w :
+    filter_heap W (force_global w) = force_global (filter_heap W w).
+  Proof.
+    apply filter_heap_map;
+      destruct w as [z|[t p g b e a|t p g b e a]|t p g b e a|ot [t p g b e a|t p g b e a] ];
+      reflexivity.
+  Qed.
+
+  Lemma filter_heap_load_word W p w :
+    filter_heap W (load_word p w) = load_word p (filter_heap W w).
+  Proof.
+    rewrite /load_word. destruct (isDRO p), (isDL p);
+      by rewrite ?filter_heap_readonly ?filter_heap_deeplocal ?filter_heap_borrow.
+  Qed.
+
   Lemma enter_cond_weakening W C p b e a :
     (□ enter_cond W C p Global b e a (fixpoint interp1)) -∗
      □ enter_cond W C p Local b e a (fixpoint interp1).
@@ -48,39 +98,31 @@ Section fundamental.
     iIntros "#Hinterp".
     destruct t; last (iApply interp_untagged; done).
     rewrite !fixpoint_interp1_eq /=.
+    iDestruct "Hinterp" as "[$ Hinterp]".
     destruct g; auto.
     iApply enter_cond_weakening;auto.
   Qed.
 
-  Local Lemma disjoint_regions_subseg b e b' e' :
-    (b <= b')%a → (e' <= e)%a →
-    disjoint_from_shadow b e ∧ disjoint_from_heap b e →
-    disjoint_from_shadow b' e' ∧ disjoint_from_heap b' e'.
+  Lemma heap_cap_valid_perm W p p' b e :
+    PermFlowsTo p' p -> heap_cap_valid W p b e -> heap_cap_valid W p' b e.
   Proof.
-    intros Hb He [Hshadow Hheap].
-    rewrite /disjoint_from_shadow elem_of_disjoint in Hshadow.
-    rewrite /disjoint_from_heap elem_of_disjoint in Hheap.
-    rewrite /disjoint_from_shadow /disjoint_from_heap !elem_of_disjoint.
-    split; intros a Ha Hregion.
-    - eapply Hshadow; last exact Hregion.
-      apply elem_of_finz_seq_between in Ha.
-      apply elem_of_finz_seq_between; solve_addr.
-    - eapply Hheap; last exact Hregion.
-      apply elem_of_finz_seq_between in Ha.
-      apply elem_of_finz_seq_between; solve_addr.
+    intros Hflow Hvalid Hnonempty. specialize (Hvalid Hnonempty).
+    move: Hvalid. rewrite /heap_cap_live.
+    destruct (is_heap_address b); last done.
+    destruct (heap_lookup_addr (heap_std W) b) as [ [base obj] | ]; last done.
+    destruct (alloc_object_status obj); last done.
+    intros [He Hexec]. split; eauto using notexecuteAllowed_flowsfrom.
   Qed.
 
-  Lemma interp_weakeningEO W C t p p' g g' b b' e e' a a' :
+  Lemma interp_weakening_same_bounds W C t p p' g g' b e a a' :
     isO p = false →
     isO p' = false →
-    (b <= b')%a ->
-    (e' <= e)%a ->
     PermFlowsTo p' p ->
     LocalityFlowsTo g' g ->
     interp W C (WCap t p g b e a) -∗
-    interp W C (WCap t p' g' b' e' a').
+    interp W C (WCap t p' g' b e a').
   Proof.
-    intros HpnotO HpnotO' Hb He Hp Hl. iIntros "HA".
+    intros HpnotO HpnotO' Hp Hl. iIntros "HA".
     destruct t; last (iApply interp_untagged; done).
     rewrite !fixpoint_interp1_eq !interp1_eq.
     rewrite HpnotO HpnotO'.
@@ -88,10 +130,10 @@ Section fundamental.
     replace (has_sreg_access p')
       with false by (symmetry; eapply nothas_sreg_access_flowsfrom; eauto).
     iDestruct "HA" as "[#A %Hconditions]".
-    destruct Hconditions as [Hpwl_cond Hregions].
-    pose proof (disjoint_regions_subseg _ _ _ _ Hb He Hregions) as Hregions'.
+    destruct Hconditions as [Hpwl_cond [Hshadow Hheap] ].
+    have Hheap' := heap_cap_valid_perm W p p' b e Hp Hheap.
     iSplit; cycle 1.
-    { iPureIntro. split; last exact Hregions'.
+    { iPureIntro. split; last by split.
       case_eq (isWL p'); intros Hpwl'; auto.
       pose proof (isWL_flowsto p' p Hp Hpwl') as Hpwl.
       rewrite Hpwl in Hpwl_cond.
@@ -105,10 +147,8 @@ Section fundamental.
       destruct g; try congruence.
       destruct g'; simpl in Hl; try tauto.
       clear Hl Hpwl_cond.
-      destruct (decide (b' < e')%a) as [Hbe'|Hbe']; cycle 1.
-      { rewrite (finz_seq_between_empty b' e'); auto; solve_addr. }
-      rewrite (isWithin_finz_seq_between_decomposition b' e' b e); last solve_addr.
-      rewrite !big_sepL_app; iDestruct "A" as "[_ [A _]]".
+      destruct (decide (b < e)%a) as [Hbe|Hbe]; cycle 1.
+      { rewrite (finz_seq_between_empty b e); auto; solve_addr. }
       iApply (big_sepL_impl with "A"); auto.
       iModIntro; iIntros (k x Hx) "Hw".
       iDestruct "Hw" as (p'' φ Hflp'' Hpersφ) "(Hrel & Hzcond & Hrcond & Hwcond & #HmonoR & %Hstate)".
@@ -118,10 +158,8 @@ Section fundamental.
       iExists p'',φ; iFrame "∗%#".
     - case_eq (isWL p); intros Hpwl; auto; rewrite Hpwl in Hpwl_cond; simplify_eq.
       + destruct g' ; inv Hl.
-        destruct (decide (b' < e')%a) as [Hbe'|Hbe']; cycle 1.
-        { rewrite (finz_seq_between_empty b' e'); auto; solve_addr. }
-        rewrite (isWithin_finz_seq_between_decomposition b' e' b e); last solve_addr.
-        rewrite !big_sepL_app; iDestruct "A" as "[_ [A _]]".
+        destruct (decide (b < e)%a) as [Hbe|Hbe]; cycle 1.
+        { rewrite (finz_seq_between_empty b e); auto; solve_addr. }
         iApply (big_sepL_impl with "A"); auto.
         iModIntro; iIntros (k x Hx) "Hw".
         iDestruct "Hw" as (p'' φ Hflp'' Hpersφ) "(Hrel & Hzcond & Hrcond & Hwcond & #HmonoR & %Hstate)".
@@ -130,10 +168,8 @@ Section fundamental.
         assert (region_state_nwl W x Local)
           as Hstate' by (cbn in * ; naive_solver).
         iExists p'',φ; iFrame "∗%#".
-      + destruct (decide (b' < e')%a) as [Hbe'|Hbe']; cycle 1.
-        { rewrite (finz_seq_between_empty b' e'); auto; solve_addr. }
-        rewrite (isWithin_finz_seq_between_decomposition b' e' b e); last solve_addr.
-        rewrite !big_sepL_app; iDestruct "A" as "[_ [A _]]".
+      + destruct (decide (b < e)%a) as [Hbe|Hbe]; cycle 1.
+        { rewrite (finz_seq_between_empty b e); auto; solve_addr. }
         iApply (big_sepL_impl with "A"); auto.
         iModIntro; iIntros (k x Hx) "Hw".
         iDestruct "Hw" as (p'' φ Hflp'' Hpersφ) "(Hrel & Hzcond & Hrcond & Hwcond & #HmonoR & %Hstate)".
@@ -142,91 +178,6 @@ Section fundamental.
         assert (region_state_nwl W x g')
           as Hstate' by (destruct g,g'; inv Hl ; cbn in * ; naive_solver).
         iExists p'',φ; iFrame "∗%#".
-  Qed.
-
-  Lemma interp_weakening W C t p p' g g' b b' e e' a a' :
-    (b <= b')%a ->
-    (e' <= e)%a ->
-    PermFlowsTo p' p ->
-    LocalityFlowsTo g' g ->
-    ftlr_IH -∗
-    interp W C (WCap t p g b e a) -∗
-    interp W C (WCap t p' g' b' e' a').
-  Proof.
-    intros Hb He Hp Hl. iIntros "#IH HA".
-    destruct t; last (iApply interp_untagged; done).
-    destruct (isO p') eqn:HpO'.
-    { rewrite !fixpoint_interp1_eq !interp1_eq HpO'; auto. }
-    destruct (isO p) eqn:HpO.
-    { eapply notisO_flowsfrom in Hp ; eauto; congruence. }
-    { iApply (interp_weakeningEO _ _ true p p' g g'); eauto. }
-  Qed.
-
-  Lemma interp_weakeningSentry W C t p g g' b b' e e' a a' :
-      isO p = false ->
-      (b <= b')%a ->
-      (e' <= e)%a ->
-      LocalityFlowsTo g' g ->
-      ftlr_IH -∗
-      interp W C (WCap t p g b e a) -∗
-      interp W C (WSentry t p g' b' e' a').
-  Proof.
-    intros HpnotO Hb He Hl.
-    iIntros "#IH HA".
-    destruct t; last (iApply interp_untagged; done).
-    rewrite !fixpoint_interp1_eq !interp1_eq /=.
-    rewrite HpnotO.
-    destruct (has_sreg_access p) eqn:HpXSR; auto.
-    iDestruct "HA" as "[#A %Hconditions]".
-    destruct Hconditions as [Hpwl_cond Hregions].
-    pose proof (disjoint_regions_subseg _ _ _ _ Hb He Hregions) as Hregions'.
-    iModIntro.
-    rewrite /enter_cond /interp_expr /=.
-    iIntros (W') "#Hfuture %g'' %Hflows !>".
-    iIntros (cstk Ws Cs regs) "#Halloc [[Hfull Hmap] (Hreg & Hworld_interp & Hcont & Hown & Hcstk & Hframe)]".
-    rewrite /interp_conf.
-    iApply ("IH" with "Halloc Hfull Hmap Hreg Hworld_interp Hcont Hframe Hown Hcstk"); eauto.
-    iModIntro. rewrite fixpoint_interp1_eq interp1_eq.
-    destruct (isO p) eqn:HpO; auto.
-    destruct (has_sreg_access p) eqn:HpXSR'; auto.
-    iSplit; cycle 1.
-    {
-      iPureIntro. split; last exact Hregions'.
-      destruct (isWL p) eqn:Hpwl; auto.
-      simplify_eq.
-      destruct g',g''; inversion Hl; inversion Hflows; auto.
-    }
-    destruct (decide (b' < e'))%a; cycle 1.
-    { rewrite (finz_seq_between_empty b' e'); auto; solve_addr. }
-    rewrite (isWithin_finz_seq_between_decomposition b' e' b e); try solve_addr.
-    rewrite !big_sepL_app. iDestruct "A" as "[_ [A2 _]]".
-    iApply (big_sepL_impl with "A2"); auto.
-    iModIntro; iIntros (k x Hx) "Hw".
-    iDestruct "Hw" as (p'' φ Hflp'' Hpersφ) "(Hrel & #Hzcond & #Hrcond & #Hwcond & #HmonoR & %Hstate)".
-    iExists p'',φ.
-    iFrame "Hrel".
-    iDestruct ( (monoReq_nwl_future W W' C g g' p p'' x φ)
-                with "[$Hfuture] [] [$HmonoR]") as "HmonoR'"; eauto.
-    repeat(iSplit; auto).
-    destruct g''.
-    - destruct g';cbn in Hflows; last done.
-      destruct g;cbn in Hl; last done.
-      iDestruct "Hfuture" as "%Hfuture".
-      destruct (isWL p); first done.
-      iPureIntro; eapply region_state_nwl_monotone_nl; eauto.
-    - destruct (isWL p); simplify_eq.
-      + destruct g';cbn in Hflows; first done.
-        iDestruct "Hfuture" as "%Hfuture".
-        iPureIntro; eapply region_state_pwl_monotone; eauto.
-      + destruct g'.
-        * destruct g;cbn in Hl; last done.
-          iDestruct "Hfuture" as "%Hfuture".
-          eapply region_state_nwl_monotone_nl in Hstate; eauto.
-          iPureIntro; by left.
-        * iDestruct "Hfuture" as "%Hfuture".
-          iPureIntro; eapply region_state_nwl_monotone; eauto.
-          destruct g; last done.
-          by left.
   Qed.
 
   Lemma interp_next_PC W C t p g b e a a' :
@@ -238,7 +189,7 @@ Section fundamental.
     destruct t; last by inversion HcorrectPC.
     inversion HcorrectPC as [p' g' b' e' a'' Hb' Hexec']; subst.
     assert (isO p = false) by (by eapply executeAllowed_nonO).
-    iApply interp_weakeningEO; eauto; try solve_addr; try done.
+    iApply interp_weakening_same_bounds; eauto; try solve_addr; try done.
   Qed.
 
   Lemma interp_lea W C t p g b e a a' :
@@ -247,7 +198,7 @@ Section fundamental.
     interp W C (WCap t p g b e a').
   Proof.
     iIntros (Hisno) "#Hi".
-    iApply interp_weakeningEO; eauto; try solve_addr; try done.
+    iApply interp_weakening_same_bounds; eauto; try solve_addr; try done.
   Qed.
 
   Lemma safe_to_unseal_weakening W C b e b' e':
@@ -302,6 +253,7 @@ Section fundamental.
     iIntros "Hinterp".
     destruct sb as [t p g b e a | t p g b e a]; destruct t;
       rewrite !fixpoint_interp1_eq /= /interp_sb /=; try done.
+    all: iDestruct "Hinterp" as "[Hinterp $]".
     all: iApply sts_seals_std_weaken; last iFrame.
     all: set_solver+.
   Qed.
@@ -319,7 +271,7 @@ Section fundamental.
     { destruct rx,w; cbn in *; try done.
       rewrite !fixpoint_interp1_eq //=.
     }
-    iApply interp_weakeningEO; eauto; try done; try solve_addr.
+    iApply interp_weakening_same_bounds; eauto; try done; try solve_addr.
     apply DL_flowsto.
   Qed.
 
@@ -338,7 +290,7 @@ Section fundamental.
         { destruct rx,w; cbn in *; try done.
           rewrite !fixpoint_interp1_eq //=.
         }
-        iApply interp_weakeningEO; eauto; try done; try solve_addr.
+        iApply interp_weakening_same_bounds; eauto; try done; try solve_addr.
       }
     - by iApply interp_weakening_from_sentry.
     - by iApply (interp_borrowed_sealed with "Hw").
@@ -361,7 +313,7 @@ Section fundamental.
     { destruct rx,w; cbn in *; try done.
       all: rewrite !fixpoint_interp1_eq //=.
     }
-    iApply (interp_weakeningEO with "Hw"); eauto; try done; try solve_addr.
+    iApply (interp_weakening_same_bounds with "Hw"); eauto; try done; try solve_addr.
     apply DRO_flowsto.
   Qed.
 
@@ -373,6 +325,546 @@ Section fundamental.
     - by iApply interp_readonly_word ; iApply interp_deeplocal_word ; iApply interp_borrow_word.
     - by iApply interp_readonly_word.
     - by iApply interp_deeplocal_word ; iApply interp_borrow_word.
+  Qed.
+
+  Lemma interp_in_mem_load_word W C p w :
+    interp_in_mem RWL W C w -∗ interp_in_mem p W C w.
+  Proof.
+    change (⊢ interp W C (filter_heap W w) -∗
+      interp W C (filter_heap W (load_word p w)))%I.
+    rewrite filter_heap_load_word.
+    iIntros "H". by iApply interp_load_word.
+  Qed.
+
+  Lemma interp_in_mem_unseal_payload W C ot sb :
+    interp W C (WSealed ot sb) -∗
+    interp_in_mem RWL W C (WSealable sb) -∗ interp W C (WSealable sb).
+  Proof.
+    iIntros "#Hsealed Hmem".
+    destruct sb as [t p g b e a|t p g b e a]; destruct t.
+    - destruct (isO p) eqn:Hp.
+      { iEval (rewrite fixpoint_interp1_eq interp1_eq Hp). done. }
+      iEval (rewrite fixpoint_interp1_eq /= /interp_sb Hp) in "Hsealed".
+      iDestruct "Hsealed" as "[_ %Hvalid]".
+      iEval (rewrite interp_in_mem_eq /load_word /= /filter_heap
+        /heap_authority_base /=) in "Hmem".
+      destruct (decide (b < e)%a) as [Hnonempty|Hempty]; last done.
+      specialize (Hvalid Hnonempty).
+      iEval (rewrite /heap_cap_base /memory_cap_base /=) in "Hmem".
+      rewrite /heap_cap_live in Hvalid.
+      destruct (is_heap_address b); last done.
+      destruct (heap_lookup_addr (heap_std W) b) as [ [base obj] | ]; last done.
+      iEval (cbn) in "Hmem".
+      destruct (alloc_object_status obj); done.
+    - iApply interp_untagged; done.
+    - iExact "Hmem".
+    - iApply interp_untagged; done.
+  Qed.
+
+  Lemma interp_in_mem_borrow_word W C w :
+    interp_in_mem RWL W C w -∗ interp_in_mem RWL W C (borrow w).
+  Proof.
+    change (⊢ interp W C (filter_heap W w) -∗ interp W C (filter_heap W (borrow w)))%I.
+    rewrite filter_heap_borrow. iIntros "H". by iApply interp_borrow_word.
+  Qed.
+
+  Lemma interp_in_mem_deeplocal_word W C w :
+    interp_in_mem RWL W C w -∗ interp_in_mem RWL W C (deeplocal w).
+  Proof.
+    change (⊢ interp W C (filter_heap W w) -∗ interp W C (filter_heap W (deeplocal w)))%I.
+    rewrite filter_heap_deeplocal. iIntros "H". by iApply interp_deeplocal_word.
+  Qed.
+
+  Lemma interp_in_mem_readonly_word W C w :
+    interp_in_mem RWL W C w -∗ interp_in_mem RWL W C (readonly w).
+  Proof.
+    change (⊢ interp W C (filter_heap W w) -∗ interp W C (filter_heap W (readonly w)))%I.
+    rewrite filter_heap_readonly. iIntros "H". by iApply interp_readonly_word.
+  Qed.
+
+  Lemma persistent_cond_interp_in_mem : persistent_cond (interp_in_mem RWL).
+  Proof. intros WCw; apply _. Qed.
+
+  Lemma zcond_interp_in_mem C : ⊢ zcond (interp_in_mem RWL) C.
+  Proof. iIntros "!> %W1 %W2 %z _". iApply interp_untagged; done. Qed.
+
+  Lemma wcond_interp_in_mem C : ⊢ wcond (interp_in_mem RWL) C interp.
+  Proof. iIntros "!> %W %w H". by iApply interp_to_in_mem. Qed.
+
+  Lemma rcond_interp_in_mem C p : ⊢ rcond (interp_in_mem RWL) C p interp.
+  Proof. iIntros "!> %W %w H". by iApply interp_in_mem_load_word. Qed.
+
+  (* Lemmas about interp  *)
+
+  Lemma interp_int W C n : ⊢ interp W C (WInt n).
+  Proof. iIntros. rewrite /interp fixpoint_interp1_eq //. Qed.
+
+  Lemma persistent_cond_interp : persistent_cond interp.
+  Proof.
+    intros W; apply _.
+  Qed.
+  Lemma zcond_interp C : ⊢ zcond interp C.
+  Proof. by iModIntro; iIntros (W1 W2 w) "_"; iApply interp_int. Qed.
+
+  Lemma wcond_interp C : ⊢ wcond interp C interp.
+  Proof. by iModIntro; iIntros (W1 w) "?". Qed.
+
+  Lemma rcond_interp C p : ⊢ rcond interp C p interp.
+  Proof. iModIntro; iIntros (W1 w) "H".
+    iApply interp_load_in_mem. by iApply interp_load_word. Qed.
+
+  Lemma monoReq_interp_in_mem (W : WORLD) (C : CmptName) (a : Addr) (p : Perm) (ρ : region_type) :
+    (std W) !! a = Some ρ
+    -> (ρ = Permanent -> isWL p = false)
+    -> ⊢ monoReq W C a p (interp_in_mem RWL).
+  Proof.
+    intros Hstd_a Hρ.
+    rewrite /monoReq Hstd_a.
+    destruct ρ; try done.
+    - destruct (isWL p) eqn:Hwl.
+      + iIntros (w W0 W1 Hrelated Hwf); iModIntro.
+        iIntros "Hinterp".
+        iApply interp_in_mem_monotone; eauto.
+      + destruct (isDL p) eqn:Hdl.
+        * iIntros (w W0 W1 Hrelated Hwf); iModIntro.
+          iIntros "Hinterp".
+          iApply interp_in_mem_monotone; eauto.
+        * iIntros (w HcanStore W0 W1 Hrelated Hwf); iModIntro.
+          iIntros "Hinterp".
+          iApply (interp_in_mem_monotone_nl W0 W1 C RWL w with "Hinterp"); [exact Hwf|exact Hrelated|].
+          cbn. by eapply canStore_global_nonisWL.
+    - ospecialize (Hρ _); first done.
+      iIntros (w HcanStore W0 W1 Hrelated Hwf); iModIntro.
+      iIntros "Hinterp".
+      iApply (interp_in_mem_monotone_nl W0 W1 C RWL w with "Hinterp"); [exact Hwf|exact Hrelated|].
+      cbn. by eapply canStore_global_nonisWL.
+  Qed.
+
+  Lemma future_priv_mono_interp_z (C : CmptName) (z : Z) :
+    ⊢ future_priv_mono C interpC (WInt z).
+  Proof.
+    iModIntro.
+    iIntros (W W') "%Hrelated %Hwf Hinterp".
+    rewrite /=.
+    iEval (rewrite fixpoint_interp1_eq);done.
+  Qed.
+
+  Lemma future_pub_mono_interp_z (C : CmptName) (z : Z) :
+    ⊢ future_pub_mono C interpC (WInt z).
+  Proof.
+    iModIntro.
+    iIntros (W W') "%Hrelated %Hwf Hinterp".
+    rewrite /=.
+    iEval (rewrite fixpoint_interp1_eq); done.
+  Qed.
+
+  Lemma future_priv_mono_interp_in_mem_z C z :
+    ⊢ future_priv_mono C interp_in_memC (WInt z).
+  Proof. iIntros "!> %W %W' %Hrelated %Hwf _". iApply interp_int. Qed.
+
+  Lemma future_pub_mono_interp_in_mem_z C z :
+    ⊢ future_pub_mono C interp_in_memC (WInt z).
+  Proof. iIntros "!> %W %W' %Hrelated %Hwf _". iApply interp_int. Qed.
+
+  Lemma future_priv_mono_interp_in_mem_global (C : CmptName) (t : bool) (p : Perm) (b e a : Addr) :
+    ⊢ future_priv_mono C interp_in_memC (WCap t p Global b e a).
+  Proof.
+    iModIntro.
+    iIntros (W W') "%Hrelated %Hwf Hinterp".
+    rewrite /=.
+    iApply (interp_in_mem_monotone_nl W W' C RWL (WCap t p Global b e a) with "Hinterp"); [exact Hwf|exact Hrelated|].
+    by destruct t.
+  Qed.
+
+  (* interp_in_mem_dl *)
+  Program Definition interp_in_mem_dl : V :=
+    (λne (W : WORLD) (B : leibnizO CmptName) (v : leibnizO Word)
+     , (interp_in_mem RWL W B (deeplocal (borrow v)))%I).
+  Solve All Obligations with solve_proper.
+
+  Lemma future_pub_mono_interp_in_mem_dl C w:
+    ⊢ future_pub_mono C (safeC interp_in_mem_dl) w.
+  Proof.
+    iIntros "!>" (W W' Hrelated Hwf) "H"; cbn.
+    iApply interp_in_mem_monotone; eauto.
+  Qed.
+
+  Lemma persistent_cond_interp_in_mem_dl : persistent_cond interp_in_mem_dl.
+  Proof. intros W; apply _. Qed.
+
+  Lemma interp_in_mem_dl_int W C n : ⊢ interp_in_mem_dl W C (WInt n).
+  Proof. iIntros; cbn; iApply interp_int. Qed.
+
+  Lemma zcond_interp_in_mem_dl C : ⊢ zcond interp_in_mem_dl C.
+  Proof. by iModIntro; iIntros (W1 W2 w) "_"; iApply interp_int. Qed.
+
+  Lemma wcond_interp_in_mem_dl C : ⊢ wcond interp_in_mem_dl C interp.
+  Proof. iIntros "!> %W %w H". iApply interp_to_in_mem. by iApply interp_deeplocal_word; iApply interp_borrow_word. Qed.
+
+  Lemma rcond_interp_in_mem_dl C p : isDL p = true -> ⊢ rcond interp_in_mem_dl C p interp.
+  Proof.
+    iIntros (Hp) "!> %W %w H".
+    rewrite /interp_in_mem_pre /load_word /= Hp.
+    destruct (isDRO p); last done.
+    by iApply interp_in_mem_readonly_word.
+  Qed.
+
+  Lemma mono_pub_interp_in_mem_dl C : ⊢ mono_pub C (safeC interp_in_mem_dl).
+  Proof. iIntros (w) "!> %W %W' %Hrelated %Hwf H"; cbn.
+    iApply (interp_in_mem_monotone W W' C RWL (deeplocal (borrow w)) with "H"); done. Qed.
+
+  Program Definition interp_in_mem_dro_eq (w : Word) : V :=
+    (λne (W : WORLD) (B : leibnizO CmptName) (v : leibnizO Word)
+     , (⌜ v = w ⌝ ∗ interp_in_mem RWL W B (readonly w))%I).
+  Solve All Obligations with solve_proper.
+
+  Lemma persistent_cond_interp_in_mem_dro_eq (w : Word) : persistent_cond (interp_in_mem_dro_eq w).
+  Proof. intros W; apply _. Qed.
+
+  Lemma zcond_interp_in_mem_dro_eq C w : ⊢ zcond (interp_in_mem_dro_eq w) C.
+  Proof. iModIntro; iIntros (W1 W2 w') "[<- ?]"; iSplit; [done | iApply interp_int]. Qed.
+
+  Lemma rcond_interp_in_mem_dro_eq C w p : isDRO p = true -> ⊢ rcond (interp_in_mem_dro_eq w) C p interp.
+  Proof.
+    iIntros (Hp) "!> %W %w' [<- H]".
+    rewrite /interp_in_mem_pre /load_word /= Hp.
+    destruct (isDL p); last done.
+    replace (readonly (deeplocal (borrow w'))) with (deeplocal (borrow (readonly w'))).
+    + by iApply interp_in_mem_deeplocal_word; iApply interp_in_mem_borrow_word.
+    + destruct w' as [| [ t [] |] | |]; auto.
+  Qed.
+
+  (* Proving the meaning of unsealing in the LR sane. Note the use of the later in the result. *)
+  (* Proving the meaning of sealing in the LR sane *)
+  Lemma sealing_preserves_interp W C sb p g b e a :
+    permit_seal p = true ->
+    withinBounds b e a = true ->
+    interp W C (WSealable sb) -∗
+    interp W C (WSealRange true p g b e a) -∗
+    world_interp W C
+    ==∗
+    ∃ W', ⌜ related_sts_pub_world W W' ⌝ ∗
+          ⌜heap_std W = heap_std W'⌝ ∗
+          world_interp W' C ∗
+          interp W' C (WSealed a sb).
+  Proof.
+    iIntros (Hseal Hwb) "#HVsb #HVsr Hworld_interp".
+    destruct (get_tag_sealable sb) eqn:Htag.
+    2: { iModIntro. iExists W. iFrame.
+         iSplit; first (iPureIntro; apply related_sts_pub_refl_world).
+         iSplit; first done. iApply interp_untagged. done. }
+    rewrite (fixpoint_interp1_eq W C (WSealRange true _ _ _ _ _)).
+    iDestruct "HVsr" as "[Hss _]"; rewrite Hseal.
+    apply seq_between_dist_Some in Hwb.
+    iDestruct (big_sepL_elem_of_acc with "Hss") as "[HSa0 _]"; eauto.
+    { rewrite list_elem_of_lookup; eauto. }
+    iDestruct "HSa0" as "(%Po & %HPo_pers & Hsealpred & %Ha0_in_Wseals & #Hwcond_Po)".
+    rewrite elem_of_dom in Ha0_in_Wseals; destruct Ha0_in_Wseals as [ws Hws].
+    set (new_seals_words := ({[WSealable sb; borrow (WSealable sb)]} : gset Word)).
+    set ( W' := <o[ a := ( new_seals_words ∪ ws) ]o> W ).
+    assert (related_sts_pub_world W W') as Hrelated.
+    { by apply related_sts_pub_world_update_ot. }
+    iAssert ([∗ set] w0 ∈ normalise_sealed_words new_seals_words, ▷ (safeC Po) (W', C, w0))%I as "Hws".
+    {
+      subst new_seals_words.
+      rewrite normalise_sealed_words_union !normalise_sealed_words_singleton; cbn.
+      rewrite force_global_borrow_sb.
+      replace ( {[WSealable (force_global_sb sb); WSealable (force_global_sb sb)]} ) with
+        ({[WSealable (force_global_sb sb)]} : gset Word) by set_solver+.
+      rewrite big_sepS_singleton -/(force_global (WSealable sb)).
+      iNext; iApply "Hwcond_Po".
+      iApply (interp_monotone_same_heap with "[%] [$HVsb]"); [reflexivity|eauto].
+    }
+    iMod (world_interp_sealing_update with "Hsealpred Hws Hworld_interp") as "(Hworld_interp & #Hstd_seals)"; eauto.
+    subst W'.
+    iModIntro.
+    iExists _. iSplit; first done. iSplit; first done.
+    iFrame "Hworld_interp".
+    iEval (rewrite fixpoint_interp1_eq /= Htag /interp_sb).
+    iSplit.
+    - iApply sts_seals_std_weaken; last iFrame "#". set_solver+.
+    - destruct sb as [t q l b' e' a'|t q l b' e' a']; destruct t;
+        cbn in Htag; try discriminate; last done.
+      destruct (isO q) eqn:Hq; first done.
+      iDestruct (interp_cap_regions with "HVsb") as %[_ Hvalid]; first done.
+      done.
+  Qed.
+
+  Lemma unsealing_preserves_interp W C sb p0 g0 b0 e0 a0 o s:
+        permit_unseal p0 = true →
+        withinBounds b0 e0 o = true →
+        interp W C (WSealed o sb) -∗
+        interp W C (WSealRange true p0 g0 b0 e0 a0) -∗
+        world_interp_open W C s
+        -∗
+        ▷ (interp W C (WSealable (machine_word.unseal g0 sb)) ∗
+           world_interp_open W C s).
+  Proof.
+    iIntros (Hpseal Hwb) "#HVsd #HVsr Hworld_interp".
+    iPoseProof "HVsd" as "#Hsealed_input".
+    destruct (get_tag_sealable sb) eqn:Htag.
+    2: { iNext. iFrame. iApply interp_untagged. by rewrite /= get_tag_unseal Htag. }
+    rewrite
+      (fixpoint_interp1_eq W C (WSealRange true _ _ _ _ _))
+      (fixpoint_interp1_eq W C (WSealed _ _)) /= Htag Hpseal /interp_sb.
+    iDestruct "HVsr" as "[_ Hss]".
+    iDestruct "HVsd" as "[HVsd _]".
+    apply seq_between_dist_Some in Hwb.
+    iDestruct (big_sepL_delete with "Hss") as "[HSa0 _]"; eauto.
+    iDestruct "HSa0" as (P) "( %Hpers & HsealP & %Hdom & Hrcond)".
+    assert (∀ WCv : WORLD * CmptName * Word, Persistent (safeC P WCv)) as Hpers'.
+    { intros [ [W0 C0] w0 ]; rewrite //=; eapply (Hpers (W0, C0, w0)). }
+    iAssert (sts_seals_std C o {[WSealable sb]}) as "#HVsd'".
+    { iApply sts_seals_std_weaken; last iFrame "HVsd"; last set_solver+. }
+    iDestruct (world_interp_open_seal_pred_singleton with "HsealP HVsd' Hworld_interp") as "(Hworld_interp & #HP)".
+    iNext.
+    rewrite /=.
+    iFrame.
+    destruct g0.
+    - rewrite unseal_global.
+      iApply (interp_in_mem_unseal_payload W C o sb with "[Hsealed_input]").
+      { iEval (rewrite fixpoint_interp1_eq /= Htag /interp_sb). done. }
+      by iApply "Hrcond".
+    - rewrite unseal_local.
+      iApply (interp_borrow_word W C (WSealable sb)).
+      iApply (interp_in_mem_unseal_payload W C o sb with "[Hsealed_input]").
+      { iEval (rewrite fixpoint_interp1_eq /= Htag /interp_sb). done. }
+      by iApply "Hrcond".
+  Qed.
+
+
+  Local Lemma disjoint_regions_subseg b e b' e' :
+    (b <= b')%a → (e' <= e)%a →
+    disjoint_from_shadow b e ∧ disjoint_from_heap b e →
+    disjoint_from_shadow b' e' ∧ disjoint_from_heap b' e'.
+  Proof.
+    intros Hb He [Hshadow Hheap].
+    rewrite /disjoint_from_shadow elem_of_disjoint in Hshadow.
+    rewrite /disjoint_from_heap elem_of_disjoint in Hheap.
+    rewrite /disjoint_from_shadow /disjoint_from_heap !elem_of_disjoint.
+    split; intros a Ha Hregion.
+    - eapply Hshadow; last exact Hregion.
+      apply elem_of_finz_seq_between in Ha.
+      apply elem_of_finz_seq_between; solve_addr.
+    - eapply Hheap; last exact Hregion.
+      apply elem_of_finz_seq_between in Ha.
+      apply elem_of_finz_seq_between; solve_addr.
+  Qed.
+
+  Lemma heap_cap_valid_subseg W p b e b' e' :
+    heap_wf (heap_std W) -> (b <= b')%a -> (e' <= e)%a ->
+    heap_cap_valid W p b e -> heap_cap_valid W p b' e'.
+  Proof.
+    intros Hwf Hb He Hvalid Hnonempty.
+    specialize (Hvalid ltac:(solve_addr)).
+    rewrite /heap_cap_live in Hvalid |- *.
+    destruct (is_heap_address b) eqn:Hbheap.
+    - destruct (heap_lookup_addr (heap_std W) b) as [ [base obj] | ] eqn:Hlookup;
+        last contradiction.
+      destruct (alloc_object_status obj) eqn:Hstatus; last contradiction.
+      destruct Hvalid as [Hend Hexec].
+      destruct (is_heap_address b') eqn:Hbheap'.
+      + destruct (heap_lookup_addr_sound _ _ _ _ Hlookup) as [Hobj Hcontains].
+        assert (Hlookup' : heap_lookup_addr (heap_std W) b' = Some (base,obj)).
+        { apply heap_lookup_addr_complete; auto.
+          rewrite /alloc_object_contains in Hcontains |- *. solve_addr. }
+        rewrite Hlookup' Hstatus. split; [solve_addr|done].
+      + rewrite /disjoint_from_heap elem_of_disjoint.
+        intros a Ha Hheap. apply elem_of_finz_seq_between in Ha, Hheap.
+        apply withinBounds_true_iff in Hbheap.
+        assert (is_heap_address b' = true) as Hcontra.
+        { apply withinBounds_true_iff. solve_addr. }
+        congruence.
+    - assert (Hdisjoint : disjoint_from_heap b' e').
+      { rewrite /disjoint_from_heap elem_of_disjoint in Hvalid |- *.
+        intros a Ha Hheap. eapply Hvalid; last exact Hheap.
+        apply elem_of_finz_seq_between in Ha.
+        apply elem_of_finz_seq_between. solve_addr. }
+      destruct (is_heap_address b') eqn:Hbheap'; last done.
+      exfalso. rewrite /disjoint_from_heap elem_of_disjoint in Hdisjoint.
+      apply withinBounds_true_iff in Hbheap'.
+      eapply (Hdisjoint b'); apply elem_of_finz_seq_between; solve_addr.
+  Qed.
+
+  Lemma interp_weakeningEO W C t p p' g g' b b' e e' a a' :
+    heap_wf (heap_std W) ->
+    isO p = false →
+    isO p' = false →
+    (b <= b')%a ->
+    (e' <= e)%a ->
+    PermFlowsTo p' p ->
+    LocalityFlowsTo g' g ->
+    interp W C (WCap t p g b e a) -∗
+    interp W C (WCap t p' g' b' e' a').
+  Proof.
+    intros Hwf HpnotO HpnotO' Hb He Hp Hl. iIntros "HA".
+    destruct t; last (iApply interp_untagged; done).
+    rewrite !fixpoint_interp1_eq !interp1_eq.
+    rewrite HpnotO HpnotO'.
+    destruct (has_sreg_access p) eqn:HpXSR; auto.
+    replace (has_sreg_access p')
+      with false by (symmetry; eapply nothas_sreg_access_flowsfrom; eauto).
+    iDestruct "HA" as "[A %Hconditions]".
+    destruct Hconditions as [Hpwl_cond Hregions].
+    destruct Hregions as [Hshadow Hheap].
+    assert (Hshadow' : disjoint_from_shadow b' e').
+    { rewrite /disjoint_from_shadow elem_of_disjoint in Hshadow |- *.
+      intros x Hx Hshadowx. eapply Hshadow; last exact Hshadowx.
+      apply elem_of_finz_seq_between in Hx.
+      apply elem_of_finz_seq_between. solve_addr. }
+    have Hheap' := heap_cap_valid_perm W p p' b' e' Hp
+      (heap_cap_valid_subseg W p b e b' e' Hwf Hb He Hheap).
+    have Hregions' := conj Hshadow' Hheap'.
+    iSplitL "A"; cycle 1.
+    { iPureIntro. split; last exact Hregions'.
+      case_eq (isWL p'); intros Hpwl'; auto.
+      pose proof (isWL_flowsto p' p Hp Hpwl') as Hpwl.
+      rewrite Hpwl in Hpwl_cond.
+      destruct g; try congruence.
+      destruct g'; simpl in Hl; tauto.
+    }
+
+    case_eq (isWL p'); intros Hpwl'; auto.
+    - pose proof (isWL_flowsto p' p Hp Hpwl') as Hpwl.
+      rewrite Hpwl in Hpwl_cond.
+      destruct g; try congruence.
+      destruct g'; simpl in Hl; try tauto.
+      clear Hl Hpwl_cond.
+      destruct (decide (b' < e')%a) as [Hbe'|Hbe']; cycle 1.
+      { rewrite (finz_seq_between_empty b' e'); auto; solve_addr. }
+      rewrite (isWithin_finz_seq_between_decomposition b' e' b e); last solve_addr.
+      iEval (rewrite !big_sepL_app) in "A". iDestruct "A" as "[_ [A _]]".
+      iApply (big_sepL_mono with "A").
+      iIntros (k x Hx) "Hw".
+      iDestruct "Hw" as (p'' φ Hflp'' Hpersφ) "(Hrel & Hzcond & Hrcond & Hwcond & HmonoR & %Hstate)".
+      rewrite Hpwl in Hstate.
+      assert ( PermFlowsTo p' p'')
+        as Hflp' by (eapply PermFlowsToTransitive; eauto).
+      iExists p'',φ; iFrame "∗%#".
+    - case_eq (isWL p); intros Hpwl; auto; rewrite Hpwl in Hpwl_cond; simplify_eq.
+      + destruct g' ; inv Hl.
+        destruct (decide (b' < e')%a) as [Hbe'|Hbe']; cycle 1.
+        { rewrite (finz_seq_between_empty b' e'); auto; solve_addr. }
+        rewrite (isWithin_finz_seq_between_decomposition b' e' b e); last solve_addr.
+        iEval (rewrite !big_sepL_app) in "A". iDestruct "A" as "[_ [A _]]".
+        iApply (big_sepL_mono with "A").
+        iIntros (k x Hx) "Hw".
+        iDestruct "Hw" as (p'' φ Hflp'' Hpersφ) "(Hrel & Hzcond & Hrcond & Hwcond & HmonoR & %Hstate)".
+        assert ( PermFlowsTo p' p'')
+          as Hflp' by (eapply PermFlowsToTransitive; eauto).
+        assert (region_state_nwl W x Local)
+          as Hstate' by (cbn in * ; naive_solver).
+        iExists p'',φ; iFrame "∗%#".
+      + destruct (decide (b' < e')%a) as [Hbe'|Hbe']; cycle 1.
+        { rewrite (finz_seq_between_empty b' e'); auto; solve_addr. }
+        rewrite (isWithin_finz_seq_between_decomposition b' e' b e); last solve_addr.
+        iEval (rewrite !big_sepL_app) in "A". iDestruct "A" as "[_ [A _]]".
+        iApply (big_sepL_mono with "A").
+        iIntros (k x Hx) "Hw".
+        iDestruct "Hw" as (p'' φ Hflp'' Hpersφ) "(Hrel & Hzcond & Hrcond & Hwcond & HmonoR & %Hstate)".
+        assert ( PermFlowsTo p' p'')
+          as Hflp' by (eapply PermFlowsToTransitive; eauto).
+        assert (region_state_nwl W x g')
+          as Hstate' by (destruct g,g'; inv Hl ; cbn in * ; naive_solver).
+        iExists p'',φ; iFrame "∗%#".
+  Qed.
+
+  Lemma interp_weakening W C t p p' g g' b b' e e' a a' :
+    heap_wf (heap_std W) ->
+    (b <= b')%a ->
+    (e' <= e)%a ->
+    PermFlowsTo p' p ->
+    LocalityFlowsTo g' g ->
+    ftlr_IH -∗
+    interp W C (WCap t p g b e a) -∗
+    interp W C (WCap t p' g' b' e' a').
+  Proof.
+    intros Hwf Hb He Hp Hl. iIntros "#IH HA".
+    destruct t; last (iApply interp_untagged; done).
+    destruct (isO p') eqn:HpO'.
+    { iEval (rewrite fixpoint_interp1_eq interp1_eq HpO'). done. }
+    destruct (isO p) eqn:HpO.
+    { eapply notisO_flowsfrom in Hp ; eauto; congruence. }
+    { iApply (interp_weakeningEO _ _ true p p' g g'); eauto. }
+  Qed.
+
+  Lemma interp_weakeningSentry W C t p g g' b b' e e' a a' :
+      is_heap_address b' = false ∧ disjoint_from_heap b' e' ->
+      isO p = false ->
+      (b <= b')%a ->
+      (e' <= e)%a ->
+      LocalityFlowsTo g' g ->
+      ftlr_IH -∗
+      interp W C (WCap t p g b e a) -∗
+      interp W C (WSentry t p g' b' e' a').
+  Proof.
+    intros Hsentry HpnotO Hb He Hl.
+    iIntros "#IH #HA".
+    destruct t; last (iApply interp_untagged; done).
+    iEval (rewrite fixpoint_interp1_eq /=).
+    iEval (rewrite fixpoint_interp1_eq interp1_eq) in "HA".
+    rewrite HpnotO.
+    destruct (has_sreg_access p) eqn:HpXSR; auto.
+    iDestruct "HA" as "[A %Hconditions]".
+    destruct Hconditions as [Hpwl_cond Hregions].
+    destruct Hregions as [Hshadow Hheap].
+    assert (Hregions' : disjoint_from_shadow b' e' ∧ disjoint_from_heap b' e').
+    { split; last exact (proj2 Hsentry).
+      rewrite /disjoint_from_shadow elem_of_disjoint in Hshadow |- *.
+      intros x Hx Hshadowx. eapply Hshadow; last exact Hshadowx.
+      apply elem_of_finz_seq_between in Hx.
+      apply elem_of_finz_seq_between. solve_addr. }
+    iSplit; first done.
+    iModIntro.
+    rewrite /enter_cond /interp_expr /=.
+    iIntros (W') "#Hfuture %g'' %Hflows !>".
+    iIntros (cstk Ws Cs regs) "#Halloc [[Hfull Hmap] (Hreg & Hworld_interp & Hcont & Hown & Hcstk & Hframe)]".
+    rewrite /interp_conf.
+    iApply ("IH" $! W' C cstk Ws Cs regs p g'' b' e' a'
+      with "Halloc Hfull Hmap Hreg Hworld_interp Hcont Hframe Hown Hcstk").
+    iModIntro. iEval (rewrite fixpoint_interp1_eq interp1_eq HpnotO HpXSR).
+    iSplitR; cycle 1.
+    {
+      iPureIntro. split; last (split; [exact (proj1 Hregions')|
+        apply heap_cap_valid_disjoint; exact (proj2 Hregions')]).
+      destruct (isWL p) eqn:Hpwl; auto.
+      simplify_eq.
+      destruct g',g''; inversion Hl; inversion Hflows; auto.
+    }
+    destruct (decide (b' < e'))%a; cycle 1.
+    { rewrite (finz_seq_between_empty b' e'); auto; solve_addr. }
+    rewrite (isWithin_finz_seq_between_decomposition b' e' b e); try solve_addr.
+    rewrite !big_sepL_app. iDestruct "A" as "[_ [A2 _]]".
+    iClear "IH Halloc".
+    iApply (big_sepL_impl with "A2").
+    iModIntro; iIntros (k x Hx) "Hw".
+    iDestruct "Hw" as (p'' φ Hflp'' Hpersφ) "(Hrel & #Hzcond & #Hrcond & #Hwcond & #HmonoR & %Hstate)".
+    iExists p'',φ.
+    iFrame "Hrel".
+    iDestruct ( (monoReq_nwl_future W W' C g g' p p'' x φ)
+                with "[$Hfuture] [] [$HmonoR]") as "HmonoR'"; eauto.
+    iFrame "Hrcond Hwcond HmonoR'".
+    iSplitR; first done. iSplitR; first done.
+    iSplitR; first (iNext; iExact "Hzcond").
+    destruct g''.
+    - destruct g';cbn in Hflows; last done.
+      destruct g;cbn in Hl; last done.
+      iDestruct "Hfuture" as "%Hfuture".
+      destruct (isWL p); first done.
+      iPureIntro; eapply region_state_nwl_monotone_nl; eauto.
+    - destruct (isWL p); simplify_eq.
+      + destruct g';cbn in Hflows; first done.
+        iDestruct "Hfuture" as "%Hfuture".
+        iPureIntro; eapply region_state_pwl_monotone; eauto.
+      + destruct g'.
+        * destruct g;cbn in Hl; last done.
+          iDestruct "Hfuture" as "%Hfuture".
+          eapply region_state_nwl_monotone_nl in Hstate; eauto.
+          iPureIntro; by left.
+        * iDestruct "Hfuture" as "%Hfuture".
+          iPureIntro; eapply region_state_nwl_monotone; eauto.
+          destruct g; last done.
+          by left.
   Qed.
 
   Lemma interp_weakening_word_load (W : WORLD) (C : CmptName) (p p' : Perm) v :
@@ -396,7 +888,7 @@ Section fundamental.
       { rewrite !fixpoint_interp1_eq !interp1_eq.
         by rewrite HnO.
       }
-      iApply (interp_weakeningEO with "Hinterp"); auto; try solve_addr.
+      iApply (interp_weakening_same_bounds with "Hinterp"); auto; try solve_addr.
       + eapply notisO_flowsfrom ; eauto.
         apply load_word_perm_load_flows;auto.
       + apply load_word_perm_load_flows;auto.
@@ -417,136 +909,5 @@ Section fundamental.
         destruct (isDL p); auto.
   Qed.
 
-  (* Lemmas about interp  *)
-
-  Lemma interp_int W C n : ⊢ interp W C (WInt n).
-  Proof. iIntros. rewrite /interp fixpoint_interp1_eq //. Qed.
-
-  Lemma persistent_cond_interp : persistent_cond interp.
-  Proof.
-    intros W; apply _.
-  Qed.
-  Lemma zcond_interp C : ⊢ zcond interp C.
-  Proof. by iModIntro; iIntros (W1 W2 w) "_"; iApply interp_int. Qed.
-
-  Lemma wcond_interp C : ⊢ wcond interp C interp.
-  Proof. by iModIntro; iIntros (W1 w) "?". Qed.
-
-  Lemma rcond_interp C p : ⊢ rcond interp C p interp.
-  Proof. iModIntro; iIntros (W1 w) "?"; by iApply interp_load_word. Qed.
-
-  Lemma monoReq_interp (W : WORLD) (C : CmptName) (a : Addr) (p : Perm) (ρ : region_type) :
-    (std W) !! a = Some ρ
-    -> (ρ = Permanent -> isWL p = false)
-    -> ⊢ monoReq W C a p interp.
-  Proof.
-    intros Hstd_a Hρ.
-    rewrite /monoReq Hstd_a.
-    destruct ρ; try done.
-    - destruct (isWL p) eqn:Hwl.
-      + iIntros (w W0 W1 Hrelated); iModIntro.
-        iIntros "Hinterp".
-        iApply interp_monotone; eauto.
-      + destruct (isDL p) eqn:Hdl.
-        * iIntros (w W0 W1 Hrelated); iModIntro.
-          iIntros "Hinterp".
-          iApply interp_monotone; eauto.
-        * iIntros (w W0 W1 HcanStore Hrelated); iModIntro.
-          iIntros "Hinterp".
-          iApply interp_monotone_nl; eauto.
-          iPureIntro; cbn.
-          by eapply canStore_global_nonisWL.
-    - ospecialize (Hρ _); first done.
-      iIntros (w W0 W1 HcanStore Hrelated); iModIntro.
-      iIntros "Hinterp".
-      iApply interp_monotone_nl; eauto.
-      iPureIntro; cbn.
-      by eapply canStore_global_nonisWL.
-  Qed.
-
-  Lemma future_priv_mono_interp_z (C : CmptName) (z : Z) :
-    ⊢ future_priv_mono C interpC (WInt z).
-  Proof.
-    iModIntro.
-    iIntros (W W') "%Hrelated Hinterp".
-    rewrite /=.
-    iEval (rewrite fixpoint_interp1_eq);done.
-  Qed.
-
-  Lemma future_pub_mono_interp_z (C : CmptName) (z : Z) :
-    ⊢ future_pub_mono C interpC (WInt z).
-  Proof.
-    iModIntro.
-    iIntros (W W') "%Hrelated Hinterp".
-    rewrite /=.
-    iEval (rewrite fixpoint_interp1_eq); done.
-  Qed.
-
-  Lemma future_priv_mono_interp_global (C : CmptName) (t : bool) (p : Perm) (b e a : Addr) :
-    ⊢ future_priv_mono C interpC (WCap t p Global b e a).
-  Proof.
-    iModIntro.
-    iIntros (W W') "%Hrelated Hinterp".
-    rewrite /=.
-    iApply interp_monotone_nl_cap; eauto.
-    by destruct t.
-  Qed.
-
-  (* interp_dl *)
-  Program Definition interp_dl : V :=
-    (λne (W : WORLD) (B : leibnizO CmptName) (v : leibnizO Word)
-     , (interp W B (deeplocal (borrow v)))%I).
-  Solve All Obligations with solve_proper.
-
-  Lemma future_pub_mono_interp_dl C w:
-    ⊢ future_pub_mono C (safeC interp_dl) w.
-  Proof.
-    iIntros "!>" (W W' Hrelated) "H"; cbn.
-    iApply interp_monotone; eauto.
-  Qed.
-
-  Lemma persistent_cond_interp_dl : persistent_cond interp_dl.
-  Proof. intros W; apply _. Qed.
-
-  Lemma interp_dl_int W C n : ⊢ interp_dl W C (WInt n).
-  Proof. iIntros; cbn; iApply interp_int. Qed.
-
-  Lemma zcond_interp_dl C : ⊢ zcond interp_dl C.
-  Proof. by iModIntro; iIntros (W1 W2 w) "_"; iApply interp_int. Qed.
-
-  Lemma wcond_interp_dl C : ⊢ wcond interp_dl C interp.
-  Proof. iIntros "!> %W %w H". by iApply interp_deeplocal_word; iApply interp_borrow_word. Qed.
-
-  Lemma rcond_interp_dl C p : isDL p = true -> ⊢ rcond interp_dl C p interp.
-  Proof.
-    iIntros (Hp) "!> %W %w H".
-    rewrite /load_word /= Hp.
-    destruct (isDRO p); last done.
-    by iApply interp_readonly_word.
-  Qed.
-
-  Lemma mono_pub_interp_dl C : ⊢ mono_pub C (safeC interp_dl).
-  Proof. iIntros (?) "!> %W %W' %Hrelated H"; cbn. iApply interp_monotone; auto. Qed.
-
-  Program Definition interp_dro_eq (w : Word) : V :=
-    (λne (W : WORLD) (B : leibnizO CmptName) (v : leibnizO Word)
-     , (⌜ v = w ⌝ ∗ interp W B (readonly w))%I).
-  Solve All Obligations with solve_proper.
-
-  Lemma persistent_cond_interp_dro_eq (w : Word) : persistent_cond (interp_dro_eq w).
-  Proof. intros W; apply _. Qed.
-
-  Lemma zcond_interp_dro_eq C w : ⊢ zcond (interp_dro_eq w) C.
-  Proof. iModIntro; iIntros (W1 W2 w') "[<- ?]"; iSplit; [done | iApply interp_int]. Qed.
-
-  Lemma rcond_interp_dro_eq C w p : isDRO p = true -> ⊢ rcond (interp_dro_eq w) C p interp.
-  Proof.
-    iIntros (Hp) "!> %W %w' [<- H]".
-    rewrite /load_word /= Hp.
-    destruct (isDL p); last done.
-    replace (readonly (deeplocal (borrow w'))) with (deeplocal (borrow (readonly w'))).
-    + by iApply interp_deeplocal_word; iApply interp_borrow_word.
-    + destruct w' as [| [ t [] |] | |]; auto.
-  Qed.
 
 End fundamental.
