theories/model/world_interp_allocation_compartments.v
@@ -201,14 +201,14 @@ Section region_alloc_cmpt.
 
     (
       (
-        ([∗ list] k ∈ (imports_addrs++code_addrs), rel C k RX interpC) ∗
-        ([∗ list] k ∈ (data_addrs), rel C k RW interpC) ∗
+        ([∗ list] k ∈ (imports_addrs++code_addrs), rel C k RX interp_in_memC) ∗
+        ([∗ list] k ∈ (data_addrs), rel C k RW interp_in_memC) ∗
         world_interp_open Winter C imports_addrs
       )
       ==∗
       world_interp_open Wfinal C imports_addrs ∗
-      ([∗ list] v ∈ cmpt_imports C_cmpt, interpC (Wfinal, C, v) ∗ future_priv_mono C interpC v) ∗
-      ([∗ set] v ∈ exported_entries_sealed C_cmpt, interp Wfinal C v)
+      ([∗ list] v ∈ cmpt_imports C_cmpt, interp_in_memC (Wfinal, C, v) ∗ future_priv_mono C interp_in_memC v) ∗
+      ([∗ set] v ∈ exported_entries_sealed C_cmpt, interp_in_mem RWL Wfinal C v)
     ) -∗
 
     world_interp W C
@@ -218,8 +218,8 @@ Section region_alloc_cmpt.
     world_interp Wfinal C ∗
     interp Wfinal C pcc_cap ∗
     interp Wfinal C cgp_cap ∗
-    ([∗ list] v ∈ cmpt_imports C_cmpt, interp Wfinal C v) ∗
-    ([∗ set] v ∈ exported_entries_sealed C_cmpt, interp Wfinal C v)
+    ([∗ list] v ∈ cmpt_imports C_cmpt, interp_in_mem RWL Wfinal C v) ∗
+    ([∗ set] v ∈ exported_entries_sealed C_cmpt, interp_in_mem RWL Wfinal C v)
   .
   Proof.
     intros * Himports Hcode Hdata C_code C_data.
@@ -227,12 +227,27 @@ Section region_alloc_cmpt.
     pose proof (cmpt_pcc_disjoint_from_heap C_cmpt) as Hpcc_heap.
     pose proof (cmpt_cgp_disjoint_from_shadow C_cmpt) as Hcgp_shadow.
     pose proof (cmpt_cgp_disjoint_from_heap C_cmpt) as Hcgp_heap.
+    assert (∀ b e, disjoint_from_heap b e ->
+      Forall (fun a => is_heap_address a = false) (finz.seq_between b e)) as Hnonheap.
+    { intros b e Hd. apply Forall_forall. intros a Ha.
+      apply not_true_is_false. intros Hheap.
+      apply withinBounds_true_iff in Hheap.
+      rewrite /disjoint_from_heap elem_of_disjoint in Hd.
+      eapply (Hd a); first exact Ha.
+      by apply elem_of_finz_seq_between. }
+    have Hpcc_nonheap := Hnonheap _ _ Hpcc_heap.
+    have Hdata_nonheap := Hnonheap _ _ Hcgp_heap.
+    rewrite (finz_seq_between_split _ (cmpt_a_code C_cmpt) _) in Hpcc_nonheap.
+    2: { pose proof (cmpt_import_size C_cmpt).
+         pose proof (cmpt_code_size C_cmpt). solve_addr. }
+    apply Forall_app in Hpcc_nonheap as [Himports_nonheap Hcode_nonheap].
     iIntros "HC_imports HC_code HC_data Himport_interp Hworld_C".
 
-    iMod (world_interp_extend_perm_sepL2 W C
+    iMod (world_interp_extend_perm_sepL2_nonheap W C
             code_addrs (cmpt_code C_cmpt)
-            RX interpC
+            RX interp_in_memC
            with "Hworld_C [HC_code]") as "(Hworld_C & #HC_code)".
+    { exact Hcode_nonheap. }
     { done. }
     { auto. }
     {
@@ -241,21 +256,21 @@ Section region_alloc_cmpt.
       - intros k v1 v2 Hv1 Hv2. cbn. iIntros; iFrame.
         pose proof (Forall_lookup_1 _ _ _ _ C_code Hv2) as Hncap.
         destruct v2; [| by inversion Hncap..].
-        rewrite fixpoint_interp1_eq /=.
-        iSplit; eauto.
-        iSplit; eauto.
+        iSplit; first done.
+        iSplit; first iApply interp_int.
         rewrite /mono_permanent.
-        iApply future_priv_mono_interp_z.
+        iApply future_priv_mono_interp_in_mem_z.
       - iFrame.
     }
 
     set ( W1 := (std_update_multiple W code_addrs Permanent)).
 
-    iMod (world_interp_extend_perm_sepL2_open _ C
+    iMod (world_interp_extend_perm_sepL2_open_nonheap _ C
             data_addrs
             (cmpt_data C_cmpt)
-            RW interpC
+            RW interp_in_memC
            with "Hworld_C [HC_data] []") as "(Hworld_C & #HC_data & _)".
+    { exact Hdata_nonheap. }
     { apply finz_seq_between_NoDup. }
     { done. }
     { apply Forall_forall. intros a Ha.
@@ -290,9 +305,10 @@ Section region_alloc_cmpt.
       iSplitL; last (iApply "IH"; eauto).
       destruct w as [| [|] | |] ; cbn in Hw; destruct Hw as [Hw|Hw]; cbn in Hw; try done
       ; [|destruct g ; last done].
-      - iSplit; last iApply future_priv_mono_interp_z.
-        by rewrite fixpoint_interp1_eq /=.
-      - iSplit; last iApply future_priv_mono_interp_global.
+      - iSplit; last iApply future_priv_mono_interp_in_mem_z.
+        iApply interp_int.
+      - iSplit; last iApply future_priv_mono_interp_in_mem_global.
+        iApply interp_to_in_mem.
         destruct tag; last (iApply interp_untagged; done).
         rewrite fixpoint_interp1_eq interp1_eq.
         destruct Hw as (Hp & Hb & He).
@@ -304,7 +320,7 @@ Section region_alloc_cmpt.
           rewrite !andb_True in Hp.
           destruct Hp as [ [ [] ] ]; done.
         }
-        iSplit; cycle 1.
+        iSplitR; cycle 1.
         { iPureIntro. split; first done.
           assert (finz.seq_between b e ⊆
             finz.seq_between (cmpt_b_cgp C_cmpt) (cmpt_e_cgp C_cmpt)) as Hbounds.
@@ -313,10 +329,11 @@ Section region_alloc_cmpt.
           split.
           - rewrite /disjoint_from_shadow in Hcgp_shadow |- *.
             set_solver+Hbounds Hcgp_shadow.
-          - rewrite /disjoint_from_heap in Hcgp_heap |- *.
+          - apply heap_cap_valid_disjoint.
+            rewrite /disjoint_from_heap in Hcgp_heap |- *.
             set_solver+Hbounds Hcgp_heap.
         }
-        iApply big_sepL_forall; cbn.
+        iApply big_sepL_intro; iModIntro.
         iIntros (k a' Ha').
         apply list_elem_of_lookup_2, elem_of_finz_seq_between in Ha'.
         assert ((cmpt_b_cgp C_cmpt) <= a' < (cmpt_e_cgp C_cmpt))%a as Ha'' by solve_addr.
@@ -327,29 +344,27 @@ Section region_alloc_cmpt.
               !! a' = Some Permanent
           ) as Ha'_W.
         { by apply std_sta_update_multiple_lookup_in_i. }
-        iExists RW, interp; cbn.
+        iExists RW, (interp_in_mem RWL); cbn.
         iSplit; first done.
-        iSplit; first (iPureIntro; apply persistent_cond_interp).
+        iSplit; first (iPureIntro; apply persistent_cond_interp_in_mem).
         iSplit; first iFrame "#".
-        iSplit; first iApply zcond_interp.
-        iSplit; first iApply rcond_interp.
-        iSplit; first iApply wcond_interp.
-        iSplit; first iApply monoReq_interp; eauto.
+        iSplit; first iApply zcond_interp_in_mem.
+        iSplit; first iApply rcond_interp_in_mem.
+        iSplit; first iApply wcond_interp_in_mem.
+        iSplitR; last done. iApply (monoReq_interp_in_mem _ _ _ RW Permanent); done.
     }
 
     set ( W2 := (std_update_multiple W1 data_addrs Permanent)).
-    (* iDestruct (sealing_map_monotone_pub _ _ W2 with "Hseals_C") as "Hseals_C". *)
-    (* { subst W2; by rewrite std_update_multiple_seals. } *)
-    (* { admit. } *)
 
-    iMod (world_interp_extend_perm_sepL2_open' _ C
+    iMod (world_interp_extend_perm_sepL2_open'_nonheap W2 C
             imports_addrs
             (cmpt_imports C_cmpt)
-            RX interpC ot_switcher
+            RX interp_in_memC ot_switcher
             (exported_entries_words C_cmpt)
             (exported_entries_sealed C_cmpt)
            with "Hworld_C HC_imports [Himport_interp]")
       as "(Hworld_C & #HC_imports & Hinterp_imports & Hinterp_exports)".
+    { exact Himports_nonheap. }
     { apply finz_seq_between_NoDup. }
     { done. }
     { apply Forall_forall.
@@ -397,19 +412,19 @@ Section region_alloc_cmpt.
 
     iSplit.
     - iEval (rewrite fixpoint_interp1_eq /=).
-      iSplit; last (iPureIntro; auto).
+      iSplitR; last (iPureIntro; split; [exact Hpcc_shadow|apply heap_cap_valid_disjoint; exact Hpcc_heap]).
       iApply big_sepL_intro; iModIntro.
       iIntros (k a Ha).
-      iExists RX, interp.
+      iExists RX, (interp_in_mem RWL).
       iEval (cbn).
       iSplit; first done.
-      iSplit; first (iPureIntro ; by apply persistent_cond_interp).
+      iSplit; first (iPureIntro ; by apply persistent_cond_interp_in_mem).
       iSplit.
       { apply list_elem_of_lookup_2 in Ha.
         iApply (big_sepL_elem_of with "HC_PCC"); eauto.
       }
-      iSplit; first (iNext ; by iApply zcond_interp).
-      iSplit; first (iNext ; by iApply rcond_interp).
+      iSplit; first (iNext ; by iApply zcond_interp_in_mem).
+      iSplit; first (iNext ; by iApply rcond_interp_in_mem).
       iSplit; first done.
       assert ((std Wfinal) !! a = Some Permanent).
       {
@@ -456,22 +471,21 @@ Section region_alloc_cmpt.
           rewrite std_sta_update_multiple_lookup_in_i; auto; set_solver+.
       }
       iSplit; last done.
-      iApply (monoReq_interp _ _ _ _ Permanent); done.
+      iApply (monoReq_interp_in_mem _ _ _ _ Permanent); done.
 
     - iEval (rewrite fixpoint_interp1_eq /=).
-      iSplit; last (iPureIntro; auto).
+      iSplitR; last (iPureIntro; split; [exact Hcgp_shadow|apply heap_cap_valid_disjoint; exact Hcgp_heap]).
       iApply big_sepL_intro; iModIntro.
       iIntros (k a Ha).
-      iExists RW, interp.
+      iExists RW, (interp_in_mem RWL).
       iEval (cbn).
       iSplit; first done.
-      iSplit; first (iPureIntro ; by apply persistent_cond_interp).
-      rewrite (big_sepL_lookup _ (finz.seq_between (cmpt_b_cgp C_cmpt) (cmpt_e_cgp C_cmpt))
-                 k a); eauto.
-      iFrame "HC_data".
-      iSplit; first (iNext ; by iApply zcond_interp).
-      iSplit; first (iNext ; by iApply rcond_interp).
-      iSplit; first (iNext ; by iApply wcond_interp).
+      iSplit; first (iPureIntro ; by apply persistent_cond_interp_in_mem).
+      iDestruct (big_sepL_lookup _ _ k a Ha with "HC_data") as "Hrel_data".
+      iSplit; first iExact "Hrel_data".
+      iSplit; first (iNext ; by iApply zcond_interp_in_mem).
+      iSplit; first (iNext ; by iApply rcond_interp_in_mem).
+      iSplit; first (iNext ; by iApply wcond_interp_in_mem).
       assert ((std Wfinal) !! a = Some Permanent).
       { subst Wfinal.
         apply list_elem_of_lookup_2 in Ha.
@@ -494,7 +508,7 @@ Section region_alloc_cmpt.
         rewrite std_sta_update_multiple_lookup_in_i; auto.
       }
       iSplit; last done.
-      iApply (monoReq_interp _ _ _ _ Permanent); done.
+      iApply (monoReq_interp_in_mem _ _ _ _ Permanent); done.
   Qed.
 
   Lemma alloc_compartment_interp (E : coPset) (W : WORLD) ( C_cmpt : cmpt ) (C : CmptName) :
@@ -524,8 +538,8 @@ Section region_alloc_cmpt.
       )
       ==∗
       world_interp_open Wfinal C imports_addrs ∗
-      ([∗ list] v ∈ cmpt_imports C_cmpt, interpC (Wfinal, C, v) ∗ future_priv_mono C interpC v) ∗
-      ([∗ set] v ∈ exported_entries_sealed C_cmpt, interp Wfinal C v)
+      ([∗ list] v ∈ cmpt_imports C_cmpt, interp_in_memC (Wfinal, C, v) ∗ future_priv_mono C interp_in_memC v) ∗
+      ([∗ set] v ∈ exported_entries_sealed C_cmpt, interp_in_mem RWL Wfinal C v)
     )
     -∗
 
@@ -536,8 +550,8 @@ Section region_alloc_cmpt.
     world_interp Wfinal C ∗
     interp Wfinal C pcc_cap ∗
     interp Wfinal C cgp_cap ∗
-    ([∗ list] v ∈ cmpt_imports C_cmpt, interp Wfinal C v) ∗
-    ([∗ set] v ∈ exported_entries_sealed C_cmpt, interp Wfinal C v)
+    ([∗ list] v ∈ cmpt_imports C_cmpt, interp_in_mem RWL Wfinal C v) ∗
+    ([∗ set] v ∈ exported_entries_sealed C_cmpt, interp_in_mem RWL Wfinal C v)
   .
   Proof.
     intros * Himports Hcode Hdata C_code C_data.
@@ -546,18 +560,19 @@ Section region_alloc_cmpt.
     pose proof (cmpt_cgp_disjoint_from_shadow C_cmpt) as Hcgp_shadow.
     pose proof (cmpt_cgp_disjoint_from_heap C_cmpt) as Hcgp_heap.
     iIntros "HC_imports HC_code HC_data Himport_interp Hworld_C".
-    iApply (alloc_compartment_interp_rel with "[$] [$] [$] [Himport_interp] [$]"); eauto.
+    iApply (alloc_compartment_interp_rel W C_cmpt C Himports Hcode Hdata C_code C_data
+      with "HC_imports HC_code HC_data [Himport_interp] Hworld_C").
     iIntros "(#Hrel_pcc & #Hrel_data & Hworld_C)".
 
     iAssert (interp Wfinal C pcc_cap) as "#Hinterp_pcc".
     { iEval (rewrite fixpoint_interp1_eq /=).
-      iSplit; last (iPureIntro; auto).
+      iSplitR; last (iPureIntro; split; [exact Hpcc_shadow|apply heap_cap_valid_disjoint; exact Hpcc_heap]).
       iApply big_sepL_intro; iModIntro.
       iIntros (ka a Ha).
-      iExists RX, interp.
+      iExists RX, (interp_in_mem RWL).
       iEval (cbn).
       iSplit; first done.
-      iSplit; first (iPureIntro ; by apply persistent_cond_interp).
+      iSplit; first (iPureIntro ; by apply persistent_cond_interp_in_mem).
       iSplit.
       { apply list_elem_of_lookup_2 in Ha.
         iApply (big_sepL_elem_of with "Hrel_pcc"); eauto.
@@ -566,8 +581,8 @@ Section region_alloc_cmpt.
         pose proof (cmpt_code_size C_cmpt) as HC'.
         solve_addr.
       }
-      iSplit; first (iNext ; by iApply zcond_interp).
-      iSplit; first (iNext ; by iApply rcond_interp).
+      iSplit; first (iNext ; by iApply zcond_interp_in_mem).
+      iSplit; first (iNext ; by iApply rcond_interp_in_mem).
       iSplit; first done.
       assert ((std Wfinal) !! a = Some Permanent).
       {
@@ -614,24 +629,23 @@ Section region_alloc_cmpt.
           rewrite std_sta_update_multiple_lookup_in_i; auto; set_solver+.
       }
       iSplit; last done.
-      iApply (monoReq_interp _ _ _ _ Permanent); done.
+      iApply (monoReq_interp_in_mem _ _ _ _ Permanent); done.
     }
 
     iAssert (interp Wfinal C cgp_cap) as "#Hinterp_cgp".
     { iEval (rewrite fixpoint_interp1_eq /=).
-      iSplit; last (iPureIntro; auto).
+      iSplitR; last (iPureIntro; split; [exact Hcgp_shadow|apply heap_cap_valid_disjoint; exact Hcgp_heap]).
       iApply big_sepL_intro; iModIntro.
       iIntros (ka a Ha).
-      iExists RW, interp.
+      iExists RW, (interp_in_mem RWL).
       iEval (cbn).
       iSplit; first done.
-      iSplit; first (iPureIntro ; by apply persistent_cond_interp).
-      rewrite (big_sepL_lookup _ (finz.seq_between (cmpt_b_cgp C_cmpt) (cmpt_e_cgp C_cmpt))
-                 ka a); eauto.
-      iFrame "Hrel_data".
-      iSplit; first (iNext ; by iApply zcond_interp).
-      iSplit; first (iNext ; by iApply rcond_interp).
-      iSplit; first (iNext ; by iApply wcond_interp).
+      iSplit; first (iPureIntro ; by apply persistent_cond_interp_in_mem).
+      iDestruct (big_sepL_lookup _ _ ka a Ha with "Hrel_data") as "Hrel_a".
+      iSplit; first iExact "Hrel_a".
+      iSplit; first (iNext ; by iApply zcond_interp_in_mem).
+      iSplit; first (iNext ; by iApply rcond_interp_in_mem).
+      iSplit; first (iNext ; by iApply wcond_interp_in_mem).
       assert ((std Wfinal) !! a = Some Permanent).
       { subst Wfinal.
         apply list_elem_of_lookup_2 in Ha.
@@ -654,7 +668,7 @@ Section region_alloc_cmpt.
         rewrite std_sta_update_multiple_lookup_in_i; auto.
       }
       iSplit; last done.
-      iApply (monoReq_interp _ _ _ _ Permanent); done.
+      iApply (monoReq_interp_in_mem _ _ _ _ Permanent); done.
     }
 
     iMod ("Himport_interp" with "[$Hinterp_pcc $Hinterp_cgp $Hworld_C]")
